start draft on a stateless sybloc

SyBloc/SBSemantics.v
@@ -9,9 +9,7 @@ Require Import Velus.Common.
 Require Import Velus.Operators.
 Require Import Velus.Clocks.
 Require Import Velus.RMemory.
-Require Import Velus.NLustre.NLExprSyntax.
 Require Import Velus.SyBloc.SBSyntax.
-Require Import Velus.NLustre.NLExprSemantics.
 Require Import Velus.NLustre.Stream.
 
 Module Type SBSEMANTICS
@@ -19,121 +17,458 @@ Module Type SBSEMANTICS
        (Import Op      : OPERATORS)
        (Import OpAux   : OPERATORS_AUX       Op)
        (Import Clks    : CLOCKS          Ids)
-       (Import ExprSyn : NLEXPRSYNTAX        Op)
-       (Import Syn     : SBSYNTAX        Ids Op Clks ExprSyn)
-       (Import Str     : STREAM              Op OpAux)
-       (Import ExprSem : NLEXPRSEMANTICS Ids Op OpAux Clks ExprSyn Str).
+       (Import Syn     : SBSYNTAX        Ids Op Clks)
+       (Import Str     : STREAM              Op OpAux).
 
-  (* Record mvalue := *)
-  (*   Mvalue { content_i: val; *)
-  (*            reset_i: bool *)
-  (*          }. *)
+  (** ** Environment and history *)
 
-  Record mvalues :=
-    Mvalues { content: stream val;
-              reset: stream bool
-            }.
+  (**
 
-  (* Definition memory := RMemory.memory mvalue. *)
-  Definition memories := RMemory.memory mvalues.
+An history maps variables to streams of values (the variables'
+histories). Taking a snapshot of the history at a given time yields an
+environment.
 
-  Inductive reset_regs: stream bool -> memories -> Prop :=
-    reset_regs_intro:
-      forall M rs,
-        (forall x mvs,
-            find_val x M = Some mvs ->
-            forall n, rs n = true -> mvs.(reset) n = true) ->
-        (forall x M',
-            sub_inst x M M' ->
-            reset_regs rs M') ->
-        reset_regs rs M.
+   *)
 
-  (* Definition next (n: nat) (mvs: mvalues) (v0 v: val) : Prop := *)
-  (*   mvs.(content) (S n) = (if mvs.(reset) (S n) then v0 else v). *)
+  Definition state := memory value.
+  Definition evolution := memory (stream value).
 
-  (* Inductive fby_spec: nat -> val -> value -> mvalues -> value -> Prop := *)
-  (* | fby_spec_present: *)
-  (*     forall n v0 v mvs, *)
-  (*       next n mvs v0 v -> *)
-  (*       fby_spec n v0 (present v) mv (mv.(content) n) *)
-  (* | fby_spec_absent: *)
-  (*     forall n v0 v mvs, *)
-  (*       next n mvs v0 (mvs.(content) n) -> *)
-  (*       fby_spec n v0 absent mvs absent. *)
+  Definition env := (PM.t value * PM.t state)%type.
+  Definition history := (PM.t (stream value) * PM.t evolution)%type.
 
-  Inductive mfby: ident -> val -> stream value -> memories -> stream value -> Prop :=
-    mfby_intro:
-      forall x mvs v0 ls M xs,
-        find_val x M = Some mvs ->
-        mvs.(content) 0 = v0 ->
-        (forall n, match ls n with
-              | absent =>
-                mvs.(content) (S n) = (if mvs.(reset) (S n) then v0 else mvs.(content) n)
-                /\ xs n = absent
-              | present v =>
-                mvs.(content) (S n) = (if mvs.(reset) (S n) then v0 else v)
-                /\ xs n = present (mvs.(content) n)
-              end) ->
-        mfby x v0 ls M xs.
+  (** ** Instantaneous semantics *)
 
-  Definition fby_eq (mems: PS.t) (eq: equation) : PS.t :=
-    match eq with
-    | EqFby x _ _ _ => PS.add x mems
-    | _ => mems
+  Section InstantSemantics.
+
+    Variable base: bool.
+    Variable R: env.
+    Variable S: state.
+
+    Inductive sem_var_instant: ident -> value -> Prop :=
+      Sv:
+        forall x v,
+          PM.find x (fst R) = Some v ->
+          sem_var_instant x v.
+
+    Inductive sem_last_instant: ident -> value -> Prop :=
+      Slv:
+        forall x v,
+          find_val x S = Some v ->
+          sem_last_instant x v.
+
+    Definition sem_vars_instant (xs: list ident) (vs: list value) : Prop :=
+      Forall2 sem_var_instant xs vs.
+
+    Inductive sem_clock_instant: clock -> bool -> Prop :=
+    | Sbase:
+        sem_clock_instant Cbase base
+    | Son:
+        forall ck x c b,
+          sem_clock_instant ck true ->
+          sem_var_instant x (present c) ->
+          val_to_bool c = Some b ->
+          sem_clock_instant (Con ck x b) true
+    | Son_abs1:
+        forall ck x c,
+          sem_clock_instant ck false ->
+          sem_var_instant x absent ->
+          sem_clock_instant (Con ck x c) false
+    | Son_abs2:
+        forall ck x c b,
+          sem_clock_instant ck true ->
+          sem_var_instant x (present c) ->
+          val_to_bool c = Some b ->
+          sem_clock_instant (Con ck x (negb b)) false.
+
+    Inductive sem_lexp_instant: lexp -> value -> Prop:=
+    | Sconst:
+        forall c v,
+          v = (if base then present (sem_const c) else absent) ->
+          sem_lexp_instant (Econst c) v
+    | Svar:
+        forall x v ty,
+          sem_var_instant x v ->
+          sem_lexp_instant (Evar x ty) v
+    | Slast:
+        forall x v ty,
+          sem_last_instant x v ->
+          sem_lexp_instant (Elast x ty) v
+    | Swhen_eq:
+        forall s x sc xc b,
+          sem_var_instant x (present xc) ->
+          sem_lexp_instant s (present sc) ->
+          val_to_bool xc = Some b ->
+          sem_lexp_instant (Ewhen s x b) (present sc)
+    | Swhen_abs1:
+        forall s x sc xc b,
+          sem_var_instant x (present xc) ->
+          val_to_bool xc = Some b ->
+          sem_lexp_instant s (present sc) ->
+          sem_lexp_instant (Ewhen s x (negb b)) absent
+    | Swhen_abs:
+        forall s x b,
+          sem_var_instant x absent ->
+          sem_lexp_instant s absent ->
+          sem_lexp_instant (Ewhen s x b) absent
+    | Sunop_eq:
+        forall le op c c' ty,
+          sem_lexp_instant le (present c) ->
+          sem_unop op c (typeof le) = Some c' ->
+          sem_lexp_instant (Eunop op le ty) (present c')
+    | Sunop_abs:
+        forall le op ty,
+          sem_lexp_instant le absent ->
+          sem_lexp_instant (Eunop op le ty) absent
+    | Sbinop_eq:
+        forall le1 le2 op c1 c2 c' ty,
+          sem_lexp_instant le1 (present c1) ->
+          sem_lexp_instant le2 (present c2) ->
+          sem_binop op c1 (typeof le1) c2 (typeof le2) = Some c' ->
+          sem_lexp_instant (Ebinop op le1 le2 ty) (present c')
+    | Sbinop_abs:
+        forall le1 le2 op ty,
+          sem_lexp_instant le1 absent ->
+          sem_lexp_instant le2 absent ->
+          sem_lexp_instant (Ebinop op le1 le2 ty) absent.
+
+    Definition sem_lexps_instant (les: list lexp) (vs: list value) :=
+      Forall2 sem_lexp_instant les vs.
+
+    Inductive sem_cexp_instant: cexp -> value -> Prop :=
+    | Smerge_true:
+        forall x t f c,
+          sem_var_instant x (present true_val) ->
+          sem_cexp_instant t (present c) ->
+          sem_cexp_instant f absent ->
+          sem_cexp_instant (Emerge x t f) (present c)
+    | Smerge_false:
+        forall x t f c,
+          sem_var_instant x (present false_val) ->
+          sem_cexp_instant t absent ->
+          sem_cexp_instant f (present c) ->
+          sem_cexp_instant (Emerge x t f) (present c)
+    | Smerge_abs:
+        forall x t f,
+          sem_var_instant x absent ->
+          sem_cexp_instant t absent ->
+          sem_cexp_instant f absent ->
+          sem_cexp_instant (Emerge x t f) absent
+    | Site_eq:
+        forall x t f c b ct cf,
+          sem_lexp_instant x (present c) ->
+          sem_cexp_instant t (present ct) ->
+          sem_cexp_instant f (present cf) ->
+          val_to_bool c = Some b ->
+          sem_cexp_instant (Eite x t f) (if b then present ct else present cf)
+    | Site_abs:
+        forall b t f,
+          sem_lexp_instant b absent ->
+          sem_cexp_instant t absent ->
+          sem_cexp_instant f absent ->
+          sem_cexp_instant (Eite b t f) absent
+    | Sexp:
+        forall e v,
+          sem_lexp_instant e v ->
+          sem_cexp_instant (Eexp e) v.
+
+  End InstantSemantics.
+
+  Section InstantAnnotatedSemantics.
+
+    Variable base : bool.
+    Variable R: env.
+    Variable S: state.
+
+    Inductive sem_annotated_instant {A}
+              (sem_instant: bool -> env -> state -> A -> value -> Prop)
+      : clock -> A -> value -> Prop :=
+    | Stick:
+        forall ck a c,
+          sem_instant base R S a (present c) ->
+          sem_clock_instant base R ck true ->
+          sem_annotated_instant sem_instant ck a (present c)
+    | Sabs:
+        forall ck a,
+          sem_instant base R S a absent ->
+          sem_clock_instant base R ck false ->
+          sem_annotated_instant sem_instant ck a absent.
+
+    Definition sem_laexp_instant := sem_annotated_instant sem_lexp_instant.
+    Definition sem_caexp_instant := sem_annotated_instant sem_cexp_instant.
+
+    Inductive sem_laexps_instant: clock -> list lexp -> list value -> Prop:=
+    | SLticks:
+        forall ck ces cs vs,
+          vs = map present cs ->
+          sem_lexps_instant base R S ces vs ->
+          sem_clock_instant base R ck true ->
+          sem_laexps_instant ck ces vs
+    | SLabss:
+        forall ck ces vs,
+          vs = all_absent ces ->
+          sem_lexps_instant base R S ces vs ->
+          sem_clock_instant base R ck false ->
+          sem_laexps_instant ck ces vs.
+
+  End InstantAnnotatedSemantics.
+
+  (** ** Liftings of instantaneous semantics *)
+
+  Section LiftSemantics.
+
+    Variable bk : stream bool.
+    Variable H : history.
+    Variable E : evolution.
+
+    Definition sample (n: nat) (xs: stream value) := xs n.
+    Hint Unfold sample.
+
+    Definition restr_evol (n: nat): state :=
+      mmap (sample n) E.
+
+    Definition restr_hist (n: nat): env :=
+      (PM.map (sample n) (fst H), PM.map (mmap (sample n)) (snd H)).
+    Hint Unfold restr_hist.
+
+    Definition lift {A B} (sem: bool -> env -> state -> A -> B -> Prop)
+               x (ys: stream B): Prop :=
+      forall n, sem (bk n) (restr_hist n) (restr_evol n) x (ys n).
+    Hint Unfold lift.
+
+    Definition lift' {A B} (sem: env -> A -> B -> Prop) x (ys: stream B): Prop :=
+      forall n, sem (restr_hist n) x (ys n).
+    Hint Unfold lift'.
+
+    Definition lift'' {A B} (sem: state -> A -> B -> Prop) x (ys: stream B): Prop :=
+      forall n, sem (restr_evol n) x (ys n).
+    Hint Unfold lift''.
+
+    Definition lift''' {A B} (sem: bool -> env -> A -> B -> Prop) x (ys: stream B): Prop :=
+      forall n, sem (bk n) (restr_hist n) x (ys n).
+    Hint Unfold lift'''.
+
+    Definition sem_clock (ck: clock) (xs: stream bool): Prop :=
+      lift''' sem_clock_instant ck xs.
+
+    Definition sem_var (x: ident) (xs: stream value): Prop :=
+      lift' sem_var_instant x xs.
+
+    Definition sem_last (x: ident) (xs: stream value): Prop :=
+      lift'' sem_last_instant x xs.
+
+    Definition sem_vars (x: idents) (xs: stream (list value)): Prop :=
+      lift' sem_vars_instant x xs.
+
+    Definition sem_laexp ck (e: lexp) (xs: stream value): Prop :=
+      lift (fun base R S => sem_laexp_instant base R S ck) e xs.
+
+    Definition sem_laexps (ck: clock) (e: list lexp) (xs: stream (list value)): Prop :=
+      lift (fun base R S => sem_laexps_instant base R S ck) e xs.
+
+    Definition sem_lexp (e: lexp) (xs: stream value): Prop :=
+      lift sem_lexp_instant e xs.
+
+    Definition sem_lexps (e: list lexp) (xs: stream (list value)): Prop :=
+      lift sem_lexps_instant e xs.
+
+    Definition sem_caexp ck (c: cexp) (xs: stream value): Prop :=
+      lift (fun base R S => sem_caexp_instant base R S ck) c xs.
+
+    Definition sem_cexp (c: cexp) (xs: stream value): Prop :=
+      lift sem_cexp_instant c xs.
+
+  End LiftSemantics.
+
+  (** ** Time-dependent semantics *)
+
+  Definition instant_same_clock (l : list value) : Prop :=
+    absent_list l \/ present_list l.
+
+  Definition same_clock (l_s : stream (list value)) : Prop :=
+    forall n, instant_same_clock (l_s n).
+
+  Definition clock_of (xss: stream (list value))(bs: stream bool): Prop :=
+    forall n,
+      present_list (xss n) <-> bs n = true.
+
+  Definition clock_of' (xss: stream (list value)) : stream bool :=
+    fun n => forallb (fun v => negb (v ==b absent)) (xss n).
+
+  Lemma clock_of_equiv:
+    forall xss, clock_of xss (clock_of' xss).
+  Proof.
+    split; intros H.
+    - unfold clock_of'.
+      rewrite forallb_forall.
+      intros; rewrite Bool.negb_true_iff.
+      rewrite not_equiv_decb_equiv.
+      eapply In_Forall in H; eauto.
+    - unfold clock_of' in H.
+      rewrite forallb_forall in H.
+      apply all_In_Forall; intros ** Hin E.
+      specialize (H _ Hin).
+      rewrite Bool.negb_true_iff, not_equiv_decb_equiv in H.
+      apply H; eauto.
+  Qed.
+
+  Lemma clock_of_equiv':
+    forall xss bk,
+      clock_of xss bk ->
+      bk ≈ clock_of' xss.
+  Proof.
+    intros ** H n; specialize (H n).
+    unfold clock_of'.
+    induction (xss n) as [|v]; simpl.
+    - apply H; constructor.
+    - destruct v.
+      + simpl.
+        rewrite <-Bool.not_true_iff_false, <-H.
+        inversion 1; auto.
+      + simpl.
+        apply IHl; rewrite <-H.
+        split; intro P.
+        * constructor; auto.
+          intro; discriminate.
+        * inv P; auto.
+  Qed.
+
+  (* Record mvalues := *)
+  (*   Mvalues { content: stream val; *)
+  (*             reset: stream bool *)
+  (*           }. *)
+
+  (* (* Definition memory := RMemory.memory mvalue. *) *)
+  (* Definition memories := RMemory.memory mvalues. *)
+
+  (* Inductive reset_regs: stream bool -> memories -> Prop := *)
+  (*   reset_regs_intro: *)
+  (*     forall M rs, *)
+  (*       (forall x mvs, *)
+  (*           find_val x M = Some mvs -> *)
+  (*           forall n, rs n = true -> mvs.(reset) n = true) -> *)
+  (*       (forall x M', *)
+  (*           sub_inst x M M' -> *)
+  (*           reset_regs rs M') -> *)
+  (*       reset_regs rs M. *)
+
+  (* (* Definition next (n: nat) (mvs: mvalues) (v0 v: val) : Prop := *) *)
+  (* (*   mvs.(content) (S n) = (if mvs.(reset) (S n) then v0 else v). *) *)
+
+  (* (* Inductive fby_spec: nat -> val -> value -> mvalues -> value -> Prop := *) *)
+  (* (* | fby_spec_present: *) *)
+  (* (*     forall n v0 v mvs, *) *)
+  (* (*       next n mvs v0 v -> *) *)
+  (* (*       fby_spec n v0 (present v) mv (mv.(content) n) *) *)
+  (* (* | fby_spec_absent: *) *)
+  (* (*     forall n v0 v mvs, *) *)
+  (* (*       next n mvs v0 (mvs.(content) n) -> *) *)
+  (* (*       fby_spec n v0 absent mvs absent. *) *)
+
+  (* Inductive mfby: ident -> val -> stream value -> memories -> stream value -> Prop := *)
+  (*   mfby_intro: *)
+  (*     forall x mvs v0 ls M xs, *)
+  (*       find_val x M = Some mvs -> *)
+  (*       mvs.(content) 0 = v0 -> *)
+  (*       (forall n, match ls n with *)
+  (*             | absent => *)
+  (*               mvs.(content) (S n) = (if mvs.(reset) (S n) then v0 else mvs.(content) n) *)
+  (*               /\ xs n = absent *)
+  (*             | present v => *)
+  (*               mvs.(content) (S n) = (if mvs.(reset) (S n) then v0 else v) *)
+  (*               /\ xs n = present (mvs.(content) n) *)
+  (*             end) -> *)
+  (*       mfby x v0 ls M xs. *)
+
+  (* Definition fby_eq (mems: PS.t) (eq: equation) : PS.t := *)
+  (*   match eq with *)
+  (*   | EqFby x _ _ _ => PS.add x mems *)
+  (*   | _ => mems *)
+  (*   end. *)
+
+  (* Definition fbys (eqs: list equation) : PS.t := *)
+  (*   fold_left fby_eq eqs PS.empty. *)
+
+  (* Definition inst_eq (insts: PS.t) (eq: equation) : PS.t := *)
+  (*   match eq with *)
+  (*   | EqReset _ _ i _ => PS.add i insts *)
+  (*   | EqCall _ _ _ i _ => PS.add i insts *)
+  (*   | _ => insts *)
+  (*   end. *)
+
+  (* Definition insts (eqs: list equation) : PS.t := *)
+  (*   fold_left inst_eq eqs PS.empty. *)
+
+  (* Definition well_structured_memories (eqs: list equation) (M: memories) := *)
+  (*   (forall x, *)
+  (*       find_val x M <> None <-> PS.In x (fbys eqs)) *)
+  (*   /\ forall x, *)
+  (*     find_inst x M <> None <-> PS.In x (insts eqs). *)
+
+  Definition reset_of_value (v: value) : bool :=
+    match v with
+    | present x => x ==b true_val
+    | absent => false
     end.
 
-  Definition fbys (eqs: list equation) : PS.t :=
-    fold_left fby_eq eqs PS.empty.
+  Definition reset_of (xs: stream value) : stream bool :=
+    fun n => reset_of_value (xs n).
 
-  Definition inst_eq (insts: PS.t) (eq: equation) : PS.t :=
-    match eq with
-    | EqReset _ _ i _ => PS.add i insts
-    | EqCall _ _ _ i _ => PS.add i insts
-    | _ => insts
-    end.
+  Definition reset_last (bl: block) (r: stream bool) (x: ident) (xs: stream value) :=
+    fun n => match xs n with
+          | absent => absent
+          | present _ =>
+            if r n then
+              match find_init x bl with
+              | Some c => present (sem_const c)
+              | None => absent
+              end
+            else xs n
+          end.
 
-  Definition insts (eqs: list equation) : PS.t :=
-    fold_left inst_eq eqs PS.empty.
-
-  Definition well_structured_memories (eqs: list equation) (M: memories) :=
-    (forall x,
-        find_val x M <> None <-> PS.In x (fbys eqs))
-    /\ forall x,
-      find_inst x M <> None <-> PS.In x (insts eqs).
+  Definition reset (bl: block) (r: stream bool) (E: evolution) :=
+    Mnode (Env.mapi (reset_last bl r) (values E)) (instances E).
 
   Section BlockSemantics.
 
     Variable P: program.
 
-    Inductive sem_equation: stream bool -> history -> memories -> equation -> Prop :=
-    | SEqDef:
-        forall bk H M x xs ck ce,
-          sem_var H x xs ->
-          sem_caexp bk H ck ce xs ->
-          sem_equation bk H M (EqDef x ck ce)
-    | SEqFby:
-        forall bk H M x ck c0 e xs ls,
-          sem_var H x xs ->
-          sem_laexp bk H ck e ls ->
-          mfby x (sem_const c0) ls M xs ->
-          sem_equation bk H M (EqFby x ck c0 e)
-    | SEqReset:
-        forall bk H M ck b i r rs M',
-          sem_var H r rs ->
-          sub_inst i M M' ->
-          reset_regs (reset_of rs) M' ->
-          sem_equation bk H M (EqReset ck b i r)
-    | SEqCall:
-        forall bk H M ys M' ck b i es ess oss,
-          sem_laexps bk H ck es ess ->
-          sub_inst i M M' ->
-          sem_block b M' ess oss ->
-          sem_vars H ys oss ->
-          sem_equation bk H M (EqCall ys ck b i es)
+    Inductive sem_reset: ident -> stream bool -> evolution -> evolution -> Prop :=
+      SReset:
+        forall b (r: stream bool) E E0 bl P',
+          find_block b P = Some (bl, P') ->
+          E0 = reset bl r E ->
+          sem_reset b r E E0.
 
-    with sem_block: ident -> memories -> stream (list value) -> stream (list value) -> Prop :=
+    Inductive sem_equation: stream bool -> history -> evolution -> equation -> evolution -> Prop :=
+    | SEqDef:
+        forall bk H E x xs ck ce,
+          sem_var H x xs ->
+          sem_caexp bk H E ck ce xs ->
+          sem_equation bk H E (EqDef x ck ce) E
+    | SEqNext:
+        forall bk H E E' x ck e xs ls,
+          sem_last E' x xs ->
+          sem_laexp bk H E ck e ls ->
+          sem_equation bk H E (EqNext x ck e) E'
+    | SEqReset:
+        forall bk H E s0 ck b s e ls Es E0,
+          sem_laexp bk H E ck e ls ->
+          sub_inst s E Es ->
+          sem_reset b (reset_of ls) Es E0 ->
+          PM.find s0 (snd H) = Some E0 ->
+          sem_equation bk H E (EqReset s0 ck b s e) E
+    | SEqCall:
+        forall bk H E E' s' ys ck b s es ess Es oss Es',
+          sem_laexps bk H E ck es ess ->
+          PM.find s (snd H) = Some Es ->
+          sem_block b Es ess oss Es' ->
+          sem_vars H ys oss ->
+          sub_inst s' E' Es' ->
+          sem_equation bk H E (EqCall s' ys ck b s es) E'
+
+    with sem_block: ident -> evolution -> stream (list value) -> stream (list value) -> evolution -> Prop :=
            SBlock:
-             forall b bl P' M H xss yss bk,
+             forall b bl P' E E' H xss yss bk,
                clock_of xss bk ->
                find_block b P = Some (bl, P') ->
                sem_vars H (map fst bl.(b_in)) xss ->
@@ -141,49 +476,50 @@ Module Type SBSEMANTICS
                same_clock xss ->
                same_clock yss ->
                (forall n, absent_list (xss n) <-> absent_list (yss n)) ->
-               Forall (sem_equation bk H M) bl.(b_eqs) ->
-               well_structured_memories bl.(b_eqs) M ->
-               sem_block b M xss yss.
+               Forall (fun eq => sem_equation bk H E eq E') bl.(b_eqs) ->
+               (* well_structured_memories bl.(b_eqs) M -> *)
+               sem_block b E xss yss E'.
 
   End BlockSemantics.
 
   Section sem_block_mult.
     Variable P: program.
 
-    Variable P_equation: stream bool -> history -> memories -> equation -> Prop.
-    Variable P_block: ident -> memories -> stream (list value) -> stream (list value) -> Prop.
+    Variable P_equation: stream bool -> history -> evolution -> equation -> evolution -> Prop.
+    Variable P_block: ident -> evolution -> stream (list value) -> stream (list value) -> evolution -> Prop.
 
     Hypothesis EqDefCase:
-      forall bk H M x xs ck ce,
+      forall bk H E x xs ck ce,
         sem_var H x xs ->
-        sem_caexp bk H ck ce xs ->
-        P_equation bk H M (EqDef x ck ce).
+        sem_caexp bk H E ck ce xs ->
+        P_equation bk H E (EqDef x ck ce) E.
 
-    Hypothesis EqFbyCase:
-      forall bk H M x ck c0 e xs ls,
-        sem_var H x xs ->
-        sem_laexp bk H ck e ls ->
-        mfby x (sem_const c0) ls M xs ->
-        P_equation bk H M (EqFby x ck c0 e).
+    Hypothesis EqNextCase:
+      forall bk H E E' x ck e xs ls,
+        sem_last E' x xs ->
+        sem_laexp bk H E ck e ls ->
+        P_equation bk H E (EqNext x ck e) E'.
 
     Hypothesis EqResetCase:
-      forall bk H M ck b i r rs M',
-        sem_var H r rs ->
-        sub_inst i M M' ->
-        reset_regs (reset_of rs) M' ->
-        P_equation bk H M (EqReset ck b i r).
+      forall bk H E s0 ck b s e ls Es E0,
+        sem_laexp bk H E ck e ls ->
+        sub_inst s E Es ->
+        sem_reset P b (reset_of ls) Es E0 ->
+        PM.find s0 (snd H) = Some E0 ->
+        P_equation bk H E (EqReset s0 ck b s e) E.
 
     Hypothesis EqCallCase:
-      forall bk H M ys M' ck b i es ess oss,
-        sem_laexps bk H ck es ess ->
-        sub_inst i M M' ->
-        sem_block P b M' ess oss ->
+      forall bk H E E' s' ys ck b s es ess Es oss Es',
+        sem_laexps bk H E ck es ess ->
+        PM.find s (snd H) = Some Es ->
+        sem_block P b Es ess oss Es' ->
         sem_vars H ys oss ->
-        P_block b M' ess oss ->
-        P_equation bk H M (EqCall ys ck b i es).
+        sub_inst s' E' Es' ->
+        P_block b Es ess oss Es' ->
+        P_equation bk H E (EqCall s' ys ck b s es) E'.
 
     Hypothesis BlockCase:
-      forall b bl P' M H xss yss bk,
+      forall b bl P' H E E' xss yss bk,
         clock_of xss bk ->
         find_block b P = Some (bl, P') ->
         sem_vars H (map fst bl.(b_in)) xss ->
@@ -191,24 +527,22 @@ Module Type SBSEMANTICS
         same_clock xss ->
         same_clock yss ->
         (forall n, absent_list (xss n) <-> absent_list (yss n)) ->
-        Forall (sem_equation P bk H M) bl.(b_eqs) ->
-        well_structured_memories bl.(b_eqs) M ->
-        Forall (P_equation bk H M) bl.(b_eqs) ->
-        P_block b M xss yss.
+        Forall (fun eq => sem_equation P bk H E eq E') bl.(b_eqs) ->
+        Forall (fun eq => P_equation bk H E eq E') bl.(b_eqs) ->
+        P_block b E xss yss E'.
 
     Fixpoint sem_equation_mult
-            (b: stream bool) (H: history) (M: memories) (e: equation)
-            (Sem: sem_equation P b H M e) {struct Sem}
-      : P_equation b H M e
+            (b: stream bool) (H: history) (E: evolution) (e: equation) (E': evolution)
+            (Sem: sem_equation P b H E e E') {struct Sem}
+      : P_equation b H E e E'
     with sem_block_mult
-           (f: ident) (M: memories) (xss oss: stream (list value))
-           (Sem: sem_block P f M xss oss) {struct Sem}
-         : P_block f M xss oss.
+           (f: ident) (E: evolution) (xss oss: stream (list value)) (E': evolution)
+           (Sem: sem_block P f E xss oss E') {struct Sem}
+         : P_block f E xss oss E'.
     Proof.
       - destruct Sem; eauto.
       - destruct Sem.
         eapply BlockCase; eauto.
-        match goal with H: well_structured_memories _ _ |- _ => clear H end.
         match goal with H: Forall _ _ |- _ => induction H; auto end.
     Qed.
 
@@ -219,7 +553,509 @@ Module Type SBSEMANTICS
 
   (** Morphisms properties *)
 
-  Add Parametric Morphism P b M: (sem_block P b M)
+  Add Parametric Morphism b A B sem H E : (@lift b H E A B sem)
+      with signature eq ==> @eq_str B ==> Basics.impl
+        as lift_eq_str.
+  Proof.
+    intros x xs xs' Eq Lift n.
+    rewrite <-Eq; auto.
+  Qed.
+
+  Add Parametric Morphism A B sem H : (@lift' H A B sem)
+      with signature eq ==> @eq_str B ==> Basics.impl
+        as lift'_eq_str.
+  Proof.
+    intros x xs xs' E Lift n.
+    rewrite <-E; auto.
+  Qed.
+
+  Add Parametric Morphism A B sem E : (@lift'' E A B sem)
+      with signature eq ==> @eq_str B ==> Basics.impl
+        as lift''_eq_str.
+  Proof.
+    intros x xs xs' Eq Lift n.
+    rewrite <-Eq; auto.
+  Qed.
+
+  Add Parametric Morphism b A B sem E : (@lift''' b E A B sem)
+      with signature eq ==> @eq_str B ==> Basics.impl
+        as lift'''_eq_str.
+  Proof.
+    intros x xs xs' Eq Lift n.
+    rewrite <-Eq; auto.
+  Qed.
+
+  Add Parametric Morphism : clock_of
+      with signature eq_str ==> eq ==> Basics.impl
+        as clock_of_eq_str.
+  Proof.
+    unfold clock_of. intros ** E b Pres n.
+    split; intros H.
+    - apply Pres.
+      specialize (E n).
+      induction H; rewrite E; constructor; auto.
+    - apply Pres in H.
+      specialize (E n).
+      induction H; rewrite <-E; constructor; auto.
+  Qed.
+
+  (* Add Parametric Morphism : reset_of *)
+  (*     with signature eq_str ==> eq_str *)
+  (*       as reset_of_eq_str. *)
+  (* Proof. *)
+  (*   unfold reset_of. intros ** E n. *)
+  (*   now rewrite E. *)
+  (* Qed. *)
+
+  (* Add Parametric Morphism : reset_regs *)
+  (*     with signature eq_str ==> eq ==> Basics.impl *)
+  (*       as reset_regs_eq_str. *)
+  (* Proof. *)
+  (*   intros ** E M Rst. *)
+  (*   induction Rst; constructor; eauto. *)
+  (* Qed. *)
+
+  Add Parametric Morphism : same_clock
+      with signature eq_str ==> Basics.impl
+        as same_clock_eq_str.
+  Proof.
+    unfold same_clock; intros ** E ? ?; rewrite <-E; auto.
+  Qed.
+
+  (** ** Clocking property *)
+
+  Lemma not_subrate_clock:
+    forall R ck,
+      ~ sem_clock_instant false R ck true.
+  Proof.
+    intros ** Sem; induction ck; inv Sem.
+    now apply IHck.
+  Qed.
+
+  Lemma present_not_absent_list:
+    forall xs (vs: list val),
+      instant_same_clock xs ->
+      ~ absent_list xs ->
+      present_list xs.
+  Proof.
+    intros ** Hsamexs Hnabs.
+    now destruct Hsamexs.
+  Qed.
+
+  Lemma sem_vars_gt0:
+    forall H (xs: list (ident * type)) ls,
+      0 < length xs ->
+      sem_vars H (map fst xs) ls ->
+      forall n, 0 < length (ls n).
+  Proof.
+    intros ** Hgt0 Hsem n.
+    specialize (Hsem n).
+    apply Forall2_length in Hsem.
+    rewrite map_length in Hsem.
+    now rewrite Hsem in Hgt0.
+  Qed.
+
+  Ltac assert_const_length xss :=
+    match goal with
+      H: sem_vars _ _ xss |- _ =>
+      let H' := fresh in
+      let k := fresh in
+      let k' := fresh in
+      assert (wf_streams xss)
+        by (intros k k'; pose proof H as H';
+            unfold sem_vars, lift in *;
+            specialize (H k); specialize (H' k');
+            apply Forall2_length in H; apply Forall2_length in H';
+            now rewrite H in H')
+    end.
+
+  (** ** Determinism of the semantics *)
+
+  (** *** Instantaneous semantics *)
+
+  Section InstantDeterminism.
+
+    Variable base: bool.
+    Variable R: env.
+    Variable S: state.
+
+    Lemma sem_var_instant_det:
+      forall x v1 v2,
+        sem_var_instant R x v1
+        -> sem_var_instant R x v2
+        -> v1 = v2.
+    Proof.
+      intros x v1 v2 H1 H2.
+      inversion_clear H1 as [Hf1];
+        inversion_clear H2 as [Hf2];
+        congruence.
+    Qed.
+
+    Lemma sem_last_instant_det:
+      forall x v1 v2,
+        sem_last_instant S x v1
+        -> sem_last_instant S x v2
+        -> v1 = v2.
+    Proof.
+      intros x v1 v2 H1 H2.
+      inversion_clear H1 as [Hf1];
+        inversion_clear H2 as [Hf2];
+        congruence.
+    Qed.
+
+    Lemma sem_clock_instant_det:
+      forall ck v1 v2,
+        sem_clock_instant base R ck v1
+        -> sem_clock_instant base R ck v2
+        -> v1 = v2.
+    Proof.
+      induction ck; repeat inversion 1; subst; intuition;
+        try repeat progress match goal with
+                            | H1: sem_clock_instant ?bk ?R ?ck ?l,
+                                  H2: sem_clock_instant ?bk ?R ?ck ?r |- _ =>
+                              apply IHck with (1:=H1) in H2; discriminate
+                            | H1: sem_var_instant ?R ?i (present ?l),
+                                  H2: sem_var_instant ?R ?i (present ?r) |- _ =>
+                              apply sem_var_instant_det with (1:=H1) in H2;
+                                injection H2; intro; subst
+                            | H1: val_to_bool _ = Some ?b, H2: val_to_bool _ = _ |- _ =>
+                              rewrite H1 in H2; destruct b; discriminate
+                            end.
+    Qed.
+
+    Lemma sem_lexp_instant_det:
+      forall e v1 v2,
+        sem_lexp_instant base R S e v1
+        -> sem_lexp_instant base R S e v2
+        -> v1 = v2.
+    Proof.
+      induction e (* using lexp_ind2 *);
+        try now (do 2 inversion_clear 1);
+        match goal with
+        | H1:sem_var_instant ?R ?e (present ?b1),
+             H2:sem_var_instant ?R ?e (present ?b2),
+                H3: ?b1 <> ?b2 |- _ =>
+          exfalso; apply H3;
+            cut (present (Vbool b1) = present (Vbool b2)); [now injection 1|];
+              eapply sem_var_instant_det; eassumption
+        | H1:sem_var_instant ?R ?e ?v1,
+             H2:sem_var_instant ?R ?e ?v2 |- ?v1 = ?v2 =>
+          eapply sem_var_instant_det; eassumption
+        | H1:sem_var_instant ?R ?e (present _),
+             H2:sem_var_instant ?R ?e absent |- _ =>
+          apply (sem_var_instant_det _ _ _ _ H1) in H2;
+            discriminate
+        | _ => auto
+        end.
+      - (* Econst *)
+        do 2 inversion_clear 1; destruct base; congruence.
+      - (* Ewhen *)
+        intros v1 v2 Hsem1 Hsem2.
+        inversion Hsem1; inversion Hsem2; subst;
+          repeat progress match goal with
+                          | H1:sem_lexp_instant ?b ?R ?e ?v1,
+                               H2:sem_lexp_instant ?b ?R ?e ?v2 |- _ =>
+                            apply IHe with (1:=H1) in H2
+                          | H1:sem_var_instant ?R ?i ?v1,
+                               H2:sem_var_instant ?R ?i ?v2 |- _ =>
+                            apply sem_var_instant_det with (1:=H1) in H2
+                          | H1:sem_unop _ _ _ = Some ?v1,
+                               H2:sem_unop _ _ _ = Some ?v2 |- _ =>
+                            rewrite H1 in H2; injection H2; intro; subst
+                          | Hp:present _ = present _ |- _ =>
+                            injection Hp; intro; subst
+                          | H1:val_to_bool _ = Some _,
+                               H2:val_to_bool _ = Some (negb _) |- _ =>
+                            rewrite H2 in H1; exfalso; injection H1;
+                              now apply Bool.no_fixpoint_negb
+                          end; subst; auto.
+      - (* Eunop *)
+        intros v1 v2 Hsem1 Hsem2.
+        inversion_clear Hsem1; inversion_clear Hsem2;
+          repeat progress match goal with
+                          | H1:sem_lexp_instant _ _ _ e _, H2:sem_lexp_instant _ _ _ e _ |- _ =>
+                            apply IHe with (1:=H1) in H2; inversion H2; subst
+                          | H1:sem_unop _ _ _ = _, H2:sem_unop _ _ _ = _ |- _ =>
+                            rewrite H1 in H2; injection H2; intro; subst
+                          | H1:sem_lexp_instant _ _ _ _ (present _),
+                               H2:sem_lexp_instant _ _ _ _ absent |- _ =>
+                            apply IHe with (1:=H1) in H2
+                          end; try auto.
+      - (* Ebinop *)
+        intros v1 v2 Hsem1 Hsem2.
+        inversion_clear Hsem1; inversion_clear Hsem2;
+          repeat progress match goal with
+                          | H1:sem_lexp_instant _ _ _ e1 _, H2:sem_lexp_instant _ _ _ e1 _ |- _ =>
+                            apply IHe1 with (1:=H1) in H2
+                          | H1:sem_lexp_instant _ _ _ e2 _, H2:sem_lexp_instant _ _ _ e2 _ |- _ =>
+                            apply IHe2 with (1:=H1) in H2
+                          | H1:sem_binop _ _ _ _ _ = Some ?v1,
+                               H2:sem_binop _ _ _ _ _ = Some ?v2 |- _ =>
+                            rewrite H1 in H2; injection H2; intro; subst
+                          | H:present _ = present _ |- _ => injection H; intro; subst
+                          end; subst; auto; discriminate.
+      - (* Elast *)
+        intros v1 v2 Hsem1 Hsem2.
+        inv Hsem1; inv Hsem2.
+        eapply sem_last_instant_det; eauto.
+    Qed.
+
+    Lemma sem_laexp_instant_det:
+      forall ck e v1 v2,
+        sem_laexp_instant base R S ck e v1
+        -> sem_laexp_instant base R S ck e v2
+        -> v1 = v2.
+    Proof.
+      intros ck e v1 v2.
+      do 2 inversion_clear 1;
+        match goal with
+        | H1:sem_lexp_instant _ _ _ _ _, H2:sem_lexp_instant _ _ _ _ _ |- _ =>
+          eapply sem_lexp_instant_det; eassumption
+        | H1:sem_clock_instant _ _ _ ?T, H2:sem_clock_instant _ _ _ ?F |- _ =>
+          assert (T = F) by (eapply sem_clock_instant_det; eassumption);
+            try discriminate
+        end; auto.
+    Qed.
+
+    Lemma sem_lexps_instant_det:
+      forall les cs1 cs2,
+        sem_lexps_instant base R S les cs1 ->
+        sem_lexps_instant base R S les cs2 ->
+        cs1 = cs2.
+    Proof.
+      intros les cs1 cs2. apply Forall2_det. apply sem_lexp_instant_det.
+    Qed.
+
+    Lemma sem_laexps_instant_det:
+      forall ck e v1 v2,
+        sem_laexps_instant base R S ck e v1
+        -> sem_laexps_instant base R S ck e v2
+        -> v1 = v2.
+    Proof.
+      intros until v2.
+      do 2 inversion_clear 1;
+        match goal with
+        | H1: sem_lexps_instant _ _ _ _ _, H2: sem_lexps_instant _ _ _ _ _ |- _ =>
+          eapply sem_lexps_instant_det; eauto
+        | H1:sem_clock_instant _ _ _ ?T, H2:sem_clock_instant _ _ _ ?F |- _ =>
+          let H := fresh in
+          assert (H: T = F) by (eapply sem_clock_instant_det; eassumption);
+            try discriminate H
+        end; congruence.
+    Qed.
+
+    Lemma sem_cexp_instant_det:
+      forall e v1 v2,
+        sem_cexp_instant base R S e v1
+        -> sem_cexp_instant base R S e v2
+        -> v1 = v2.
+    Proof.
+      induction e;
+        do 2 inversion_clear 1;
+        try repeat progress match goal with
+                            | H1: sem_cexp_instant ?bk ?R ?S ?e ?l,
+                                  H2: sem_cexp_instant ?bk ?R ?S ?e ?r |- _ =>
+                              apply IHe1 with (1:=H1) in H2
+                                                         || apply IHe2 with (1:=H1) in H2;
+                                injection H2; intro; subst
+                            | H1: sem_var_instant ?R ?i (present true_val),
+                                  H2: sem_var_instant ?R ?i (present false_val) |- _ =>
+                              apply sem_var_instant_det with (1:=H1) in H2;
+                                exfalso; injection H2; now apply true_not_false_val
+                            | H1: sem_lexp_instant ?bk ?R ?S ?l ?v1,
+                                  H2: sem_lexp_instant ?bk ?R ?S ?l ?v2 |- _ =>
+                              apply sem_lexp_instant_det with (1:=H1) in H2;
+                                discriminate || injection H2; intro; subst
+                            | H1: sem_var_instant ?R ?i (present _),
+                                  H2: sem_var_instant ?R ?i absent |- _ =>
+                              apply sem_var_instant_det with (1:=H1) in H2; discriminate
+                            | H1: val_to_bool _ = Some _,
+                                  H2:val_to_bool _ = Some _ |- _ =>
+                              rewrite H1 in H2; injection H2; intro; subst
+                            end; auto.
+      eapply sem_lexp_instant_det; eassumption.
+    Qed.
+
+    Lemma sem_caexp_instant_det:
+      forall ck e v1 v2,
+        sem_caexp_instant base R S ck e v1
+        -> sem_caexp_instant base R S ck e v2
+        -> v1 = v2.
+    Proof.
+      intros until v2.
+      do 2 inversion_clear 1;
+        match goal with
+        | H1: sem_cexp_instant _ _ _ _ _,
+              H2: sem_cexp_instant _ _ _ _ _ |- _ =>
+          eapply sem_cexp_instant_det; eassumption
+        | H1:sem_clock_instant _ _ _ ?T,
+             H2:sem_clock_instant _ _ _ ?F |- _ =>
+          let H := fresh in
+          assert (H: T = F) by (eapply sem_clock_instant_det; eassumption);
+            try discriminate H
+        end; congruence.
+    Qed.
+
+  End InstantDeterminism.
+
+  (** *** Lifted semantics *)
+
+  (* Section LiftDeterminism. *)
+
+(*     Variable bk : stream bool. *)
+(*     Variable H : history. *)
+
+(*     Require Import Logic.FunctionalExtensionality. *)
+
+(*     Lemma lift_det: *)
+(*       forall {A B} (P: bool -> env -> A -> B -> Prop) (bk: stream bool) *)
+(*         x (xs1 xs2 : stream B), *)
+(*         (forall b R v1 v2, P b R x v1 -> P b R x v2 -> v1 = v2) -> *)
+(*         lift bk H P x xs1 -> lift bk H P x xs2 -> xs1 = xs2. *)
+(*     Proof. *)
+(*       intros ** Hpoint H1 H2. *)
+(*       extensionality n. specialize (H1 n). specialize (H2 n). *)
+(*       eapply Hpoint; eassumption. *)
+(*     Qed. *)
+
+(*     Lemma lift'_det: *)
+(*       forall {A B} (P: env -> A -> B -> Prop) *)
+(*         x (xs1 xs2 : stream B), *)
+(*         (forall R v1 v2, P R x v1 -> P R x v2 -> v1 = v2) -> *)
+(*         lift' H P x xs1 -> lift' H P x xs2 -> xs1 = xs2. *)
+(*     Proof. *)
+(*       intros ** Hpoint H1 H2. *)
+(*       extensionality n. specialize (H1 n). specialize (H2 n). *)
+(*       eapply Hpoint; eassumption. *)
+(*     Qed. *)
+
+(*     Ltac apply_lift sem_det := *)
+(*       intros; eapply lift_det; try eassumption; *)
+(*       compute; intros; eapply sem_det; eauto. *)
+
+(*     Ltac apply_lift' sem_det := *)
+(*       intros; eapply lift'_det; try eassumption; *)
+(*       compute; intros; eapply sem_det; eauto. *)
+
+(*     Lemma sem_var_det: *)
+(*       forall x xs1 xs2, *)
+(*         sem_var H x xs1 -> sem_var H x xs2 -> xs1 = xs2. *)
+(*     Proof. *)
+(*       apply_lift' sem_var_instant_det. *)
+(*     Qed. *)
+
+(*     Lemma sem_clock_det: *)
+(*       forall ck bs1 bs2, *)
+(*         sem_clock bk H ck bs1 -> sem_clock bk H ck bs2 -> bs1 = bs2. *)
+(*     Proof. *)
+(*       apply_lift sem_clock_instant_det. *)
+(*     Qed. *)
+
+(*     Lemma sem_lexp_det: *)
+(*       forall e xs1 xs2, *)
+(*         sem_lexp bk H e xs1 -> sem_lexp bk H e xs2 -> xs1 = xs2. *)
+(*     Proof. *)
+(*       apply_lift sem_lexp_instant_det. *)
+(*     Qed. *)
+
+(*     Lemma sem_lexps_det: *)
+(*       forall les cs1 cs2, *)
+(*         sem_lexps bk H les cs1 -> *)
+(*         sem_lexps bk H les cs2 -> *)
+(*         cs1 = cs2. *)
+(*     Proof. *)
+(*       apply_lift sem_lexps_instant_det. *)
+(*     Qed. *)
+
+(*     Lemma sem_laexp_det: *)
+(*       forall ck e xs1 xs2, *)
+(*         sem_laexp bk H ck e xs1 -> sem_laexp bk H ck e xs2 -> xs1 = xs2. *)
+(*     Proof. *)
+(*       apply_lift sem_laexp_instant_det. *)
+(*     Qed. *)
+
+(*     Lemma sem_laexps_det: *)
+(*       forall ck e xs1 xs2, *)
+(*         sem_laexps bk H ck e xs1 -> sem_laexps bk H ck e xs2 -> xs1 = xs2. *)
+(*     Proof. *)
+(*       apply_lift sem_laexps_instant_det. *)
+(*     Qed. *)
+
+(*     Lemma sem_cexp_det: *)
+(*       forall c xs1 xs2, *)
+(*         sem_cexp bk H c xs1 -> sem_cexp bk H c xs2 -> xs1 = xs2. *)
+(*     Proof. *)
+(*       apply_lift sem_cexp_instant_det. *)
+(*     Qed. *)
+
+(*     Lemma sem_caexp_det: *)
+(*       forall ck c xs1 xs2, *)
+(*         sem_caexp bk H ck c xs1 -> sem_caexp bk H ck c xs2 -> xs1 = xs2. *)
+(*     Proof. *)
+(*       apply_lift sem_caexp_instant_det. *)
+(*     Qed. *)
+
+(*   (* XXX: every semantics definition, including [sem_var] which doesn't *)
+(* need it, takes a base clock value or base clock stream, except *)
+(* [sem_var_instant]. For uniformity, we may want to pass a (useless) *)
+(* clock to [sem_var_instant] too. *) *)
+
+(*   End LiftDeterminism. *)
+
+  (* Ltac sem_det := *)
+  (*   match goal with *)
+  (*   | H1: sem_clock_instant ?bk ?H ?C ?X, *)
+  (*         H2: sem_clock_instant ?bk ?H ?C ?Y |- ?X = ?Y => *)
+  (*     eapply sem_clock_instant_det; eexact H1 || eexact H2 *)
+  (*   | H1: sem_clock ?bk ?H ?C ?X, *)
+  (*         H2: sem_clock ?bk ?H ?C ?Y |- ?X = ?Y => *)
+  (*     eapply sem_clock_det; eexact H1 || eexact H2 *)
+  (*   | H1: sem_cexp_instant ?bk ?H ?C ?X, *)
+  (*         H2: sem_cexp_instant ?bk ?H ?C ?Y |- ?X = ?Y => *)
+  (*     eapply sem_cexp_instant_det; eexact H1 || eexact H2 *)
+  (*   | H1: sem_cexp ?bk ?H ?C ?X, *)
+  (*         H2: sem_cexp ?bk ?H ?C ?Y |- ?X = ?Y => *)
+  (*     eapply sem_cexp_det; eexact H1 || eexact H2 *)
+  (*   | H1: sem_lexps_instant ?bk ?H ?C ?X, *)
+  (*         H2: sem_lexps_instant ?bk ?H ?C ?Y |- ?X = ?Y => *)
+  (*     eapply sem_lexps_instant_det; eexact H1 || eexact H2 *)
+  (*   | H1: sem_lexps ?bk ?H ?C ?X, *)
+  (*         H2: sem_lexps ?bk ?H ?C ?Y |- ?X = ?Y => *)
+  (*     eapply sem_lexps_det; eexact H1 || eexact H2 *)
+  (*   | H1: sem_laexps_instant ?bk ?H ?ck ?C ?X, *)
+  (*         H2: sem_laexps_instant ?bk ?H ?ck ?C ?Y |- ?X = ?Y => *)
+  (*     eapply sem_laexps_instant_det; eexact H1 || eexact H2 *)
+  (*   | H1: sem_laexps ?bk ?H ?ck ?C ?X, *)
+  (*         H2: sem_laexps ?bk ?H ?ck ?C ?Y |- ?X = ?Y => *)
+  (*     eapply sem_laexps_det; eexact H1 || eexact H2 *)
+  (*   | H1: sem_lexp_instant ?bk ?H ?C ?X, *)
+  (*         H2: sem_lexp_instant ?bk ?H ?C ?Y |- ?X = ?Y => *)
+  (*     eapply sem_lexp_instant_det; eexact H1 || eexact H2 *)
+  (*   | H1: sem_lexp ?bk ?H ?C ?X, *)
+  (*         H2: sem_lexp ?bk ?H ?C ?Y |- ?X = ?Y => *)
+  (*     eapply sem_lexp_det; eexact H1 || eexact H2 *)
+  (*   | H1: sem_laexp_instant ?bk ?H ?CK ?C ?X, *)
+  (*         H2: sem_laexp_instant ?bk ?H ?CK ?C ?Y |- ?X = ?Y => *)
+  (*     eapply sem_laexp_instant_det; eexact H1 || eexact H2 *)
+  (*   | H1: sem_laexp ?bk ?H ?CK ?C ?X, *)
+  (*         H2: sem_laexp ?bk ?H ?CK ?C ?Y |- ?X = ?Y => *)
+  (*     eapply sem_laexp_det; eexact H1 || eexact H2 *)
+  (*   | H1: sem_var_instant ?H ?C ?X, *)
+  (*         H2: sem_var_instant ?H ?C ?Y |- ?X = ?Y => *)
+  (*     eapply sem_var_instant_det; eexact H1 || eexact H2 *)
+  (*   | H1: sem_var ?H ?C ?X, *)
+  (*         H2: sem_var ?H ?C ?Y |- ?X = ?Y => *)
+  (*     eapply sem_var_det; eexact H1 || eexact H2 *)
+  (*   end. *)
+  (* Record mvalue := *)
+  (*   Mvalue { content_i: val; *)
+  (*            reset_i: bool *)
+  (*          }. *)
+
+
+  (** Morphisms properties *)
+
+  Add Parametric Morphism P b E E': (fun xss yss => sem_block P b E xss yss E')
       with signature eq_str ==> eq_str ==> Basics.impl
         as sem_node_eq_str.
   Proof.
@@ -229,165 +1065,165 @@ Module Type SBSEMANTICS
   Qed.
 
   Lemma sem_block_wf:
-    forall P f M xss yss,
-      sem_block P f M xss yss ->
+    forall P f E E' xss yss,
+      sem_block P f E xss yss E' ->
       wf_streams xss /\ wf_streams yss.
   Proof.
     intros ** Sem; split; inv Sem;
       assert_const_length xss; assert_const_length yss; auto.
   Qed.
 
-  Lemma sem_EqCall_gt0:
-    forall P bk H M xs ck b i es,
-      sem_equation P bk H M (EqCall xs ck b i es) ->
-      0 < length xs.
-  Proof.
-    inversion_clear 1 as [| | |????????????? Block' Vars].
-    inversion_clear Block' as [??????????? Out].
-    specialize (Out 0); specialize (Vars 0); simpl in *;
-      apply Forall2_length in Out; apply Forall2_length in Vars.
-    rewrite <-Out in Vars; rewrite Vars, map_length; apply b_outgt0.
-  Qed.
+  (* Lemma sem_EqCall_gt0: *)
+  (*   forall P bk H M xs ck b i es, *)
+  (*     sem_equation P bk H M (EqCall xs ck b i es) -> *)
+  (*     0 < length xs. *)
+  (* Proof. *)
+  (*   inversion_clear 1 as [| | |????????????? Block' Vars]. *)
+  (*   inversion_clear Block' as [??????????? Out]. *)
+  (*   specialize (Out 0); specialize (Vars 0); simpl in *; *)
+  (*     apply Forall2_length in Out; apply Forall2_length in Vars. *)
+  (*   rewrite <-Out in Vars; rewrite Vars, map_length; apply b_outgt0. *)
+  (* Qed. *)
 
-  Lemma In_fold_left_fby_eq:
-    forall x eqs m,
-      PS.In x (fold_left fby_eq eqs m)
-      <-> PS.In x (fbys eqs) \/ PS.In x m.
-  Proof.
-    unfold fbys.
-    induction eqs as [|eq].
-    - split; auto.
-      destruct 1 as [H|].
-      apply not_In_empty in H; contradiction.
-      auto.
-    - split.
-      + intro H.
-        simpl; rewrite IHeqs.
-        simpl in H; apply IHeqs in H; destruct H; auto.
-        destruct eq; auto.
-        apply PS.add_spec in H.
-        destruct H.
-        rewrite H; left; right; apply PS.add_spec; intuition.
-        intuition.
-      + destruct 1 as [H|H].
-        * simpl in H; rewrite IHeqs in H; apply IHeqs; destruct H; auto.
-          right.
-          destruct eq; try (apply not_In_empty in H; contradiction).
-          simpl; apply PS.add_spec.
-          apply PS.add_spec in H; destruct H;
-            try apply not_In_empty in H; intuition.
-        * apply IHeqs; right; destruct eq; auto.
-          apply PS.add_spec; auto.
-  Qed.
+  (* Lemma In_fold_left_fby_eq: *)
+  (*   forall x eqs m, *)
+  (*     PS.In x (fold_left fby_eq eqs m) *)
+  (*     <-> PS.In x (fbys eqs) \/ PS.In x m. *)
+  (* Proof. *)
+  (*   unfold fbys. *)
+  (*   induction eqs as [|eq]. *)
+  (*   - split; auto. *)
+  (*     destruct 1 as [H|]. *)
+  (*     apply not_In_empty in H; contradiction. *)
+  (*     auto. *)
+  (*   - split. *)
+  (*     + intro H. *)
+  (*       simpl; rewrite IHeqs. *)
+  (*       simpl in H; apply IHeqs in H; destruct H; auto. *)
+  (*       destruct eq; auto. *)
+  (*       apply PS.add_spec in H. *)
+  (*       destruct H. *)
+  (*       rewrite H; left; right; apply PS.add_spec; intuition. *)
+  (*       intuition. *)
+  (*     + destruct 1 as [H|H]. *)
+  (*       * simpl in H; rewrite IHeqs in H; apply IHeqs; destruct H; auto. *)
+  (*         right. *)
+  (*         destruct eq; try (apply not_In_empty in H; contradiction). *)
+  (*         simpl; apply PS.add_spec. *)
+  (*         apply PS.add_spec in H; destruct H; *)
+  (*           try apply not_In_empty in H; intuition. *)
+  (*       * apply IHeqs; right; destruct eq; auto. *)
+  (*         apply PS.add_spec; auto. *)
+  (* Qed. *)
 
-  Lemma In_fold_left_inst_eq:
-    forall x eqs m,
-      PS.In x (fold_left inst_eq eqs m)
-      <-> PS.In x (insts eqs) \/ PS.In x m.
-  Proof.
-    unfold insts.
-    induction eqs as [|eq].
-    - split; auto.
-      destruct 1 as [H|].
-      apply not_In_empty in H; contradiction.
-      auto.
-    - split.
-      + intro H.
-        simpl; rewrite IHeqs.
-        simpl in H; apply IHeqs in H; destruct H; auto.
-        destruct eq; auto; apply PS.add_spec in H; destruct H; auto;
-          rewrite H; left; right; apply PS.add_spec; auto.
-      + destruct 1 as [H|H].
-        * simpl in H; rewrite IHeqs in H; apply IHeqs; destruct H; auto.
-          right.
-          destruct eq; try (apply not_In_empty in H; contradiction);
-            simpl; apply PS.add_spec;
-              apply PS.add_spec in H; destruct H; auto;
-                apply not_In_empty in H; contradiction.
-        * apply IHeqs; right; destruct eq; auto;
-            apply PS.add_spec; auto.
-  Qed.
+  (* Lemma In_fold_left_inst_eq: *)
+  (*   forall x eqs m, *)
+  (*     PS.In x (fold_left inst_eq eqs m) *)
+  (*     <-> PS.In x (insts eqs) \/ PS.In x m. *)
+  (* Proof. *)
+  (*   unfold insts. *)
+  (*   induction eqs as [|eq]. *)
+  (*   - split; auto. *)
+  (*     destruct 1 as [H|]. *)
+  (*     apply not_In_empty in H; contradiction. *)
+  (*     auto. *)
+  (*   - split. *)
+  (*     + intro H. *)
+  (*       simpl; rewrite IHeqs. *)
+  (*       simpl in H; apply IHeqs in H; destruct H; auto. *)
+  (*       destruct eq; auto; apply PS.add_spec in H; destruct H; auto; *)
+  (*         rewrite H; left; right; apply PS.add_spec; auto. *)
+  (*     + destruct 1 as [H|H]. *)
+  (*       * simpl in H; rewrite IHeqs in H; apply IHeqs; destruct H; auto. *)
+  (*         right. *)
+  (*         destruct eq; try (apply not_In_empty in H; contradiction); *)
+  (*           simpl; apply PS.add_spec; *)
+  (*             apply PS.add_spec in H; destruct H; auto; *)
+  (*               apply not_In_empty in H; contradiction. *)
+  (*       * apply IHeqs; right; destruct eq; auto; *)
+  (*           apply PS.add_spec; auto. *)
+  (* Qed. *)
 
-  Lemma well_structured_def:
-    forall M x ck e eqs,
-      well_structured_memories (EqDef x ck e :: eqs) M <->
-      well_structured_memories eqs M.
-  Proof.
-    split; eauto.
-  Qed.
+  (* Lemma well_structured_def: *)
+  (*   forall M x ck e eqs, *)
+  (*     well_structured_memories (EqDef x ck e :: eqs) M <-> *)
+  (*     well_structured_memories eqs M. *)
+  (* Proof. *)
+  (*   split; eauto. *)
+  (* Qed. *)
 
-  Lemma well_structured_add_inst_call:
-    forall M M' xs ck f i es eqs,
-      well_structured_memories eqs M ->
-      well_structured_memories (EqCall xs ck f i es :: eqs) (add_inst i M' M).
-  Proof.
-    intros ** WS.
-    constructor; unfold fbys, insts; simpl; split; intro H.
-    - rewrite find_val_add_inst in H; apply WS in H; auto.
-    - rewrite find_val_add_inst; apply WS in H; auto.
-    - rewrite In_fold_left_inst_eq.
-      destruct (ident_eqb x i) eqn: E;
-        [apply ident_eqb_eq in E; subst|apply ident_eqb_neq in E].
-      + right; apply PSE.MP.Dec.F.add_1; auto.
-      + rewrite find_inst_gso in H; auto.
-        apply WS in H; auto.
-    - destruct (ident_eqb x i) eqn: E;
-        [apply ident_eqb_eq in E; subst|apply ident_eqb_neq in E].
-      + rewrite find_inst_gss; intro; discriminate.
-      + rewrite find_inst_gso; auto.
-        apply WS.
-        apply In_fold_left_inst_eq in H as [|H]; auto.
-        apply PSE.MP.Dec.F.add_3 in H; auto.
-        contradict H; apply not_In_empty.
-  Qed.
+  (* Lemma well_structured_add_inst_call: *)
+  (*   forall M M' xs ck f i es eqs, *)
+  (*     well_structured_memories eqs M -> *)
+  (*     well_structured_memories (EqCall xs ck f i es :: eqs) (add_inst i M' M). *)
+  (* Proof. *)
+  (*   intros ** WS. *)
+  (*   constructor; unfold fbys, insts; simpl; split; intro H. *)
+  (*   - rewrite find_val_add_inst in H; apply WS in H; auto. *)
+  (*   - rewrite find_val_add_inst; apply WS in H; auto. *)
+  (*   - rewrite In_fold_left_inst_eq. *)
+  (*     destruct (ident_eqb x i) eqn: E; *)
+  (*       [apply ident_eqb_eq in E; subst|apply ident_eqb_neq in E]. *)
+  (*     + right; apply PSE.MP.Dec.F.add_1; auto. *)
+  (*     + rewrite find_inst_gso in H; auto. *)
+  (*       apply WS in H; auto. *)
+  (*   - destruct (ident_eqb x i) eqn: E; *)
+  (*       [apply ident_eqb_eq in E; subst|apply ident_eqb_neq in E]. *)
+  (*     + rewrite find_inst_gss; intro; discriminate. *)
+  (*     + rewrite find_inst_gso; auto. *)
+  (*       apply WS. *)
+  (*       apply In_fold_left_inst_eq in H as [|H]; auto. *)
+  (*       apply PSE.MP.Dec.F.add_3 in H; auto. *)
+  (*       contradict H; apply not_In_empty. *)
+  (* Qed. *)
 
-  Lemma well_structured_reset_call:
-    forall M xs ck f i es ck_r r eqs,
-      well_structured_memories (EqCall xs ck f i es :: eqs) M ->
-      well_structured_memories (EqReset ck_r f i r :: EqCall xs ck f i es :: eqs) M.
-  Proof.
-    inversion_clear 1 as [Vals Insts].
-    constructor; unfold fbys, insts in *; simpl in *.
-    - intro; rewrite Vals; reflexivity.
-    - intro; rewrite Insts.
-      rewrite 2 In_fold_left_inst_eq.
-      split; intros [H|H']; auto.
-      + rewrite PSE.MP.Dec.F.add_iff; auto.
-      + apply PSE.MP.Dec.F.add_iff in H' as []; auto.
-        rewrite PSE.MP.Dec.F.add_iff; auto.
-  Qed.
+  (* Lemma well_structured_reset_call: *)
+  (*   forall M xs ck f i es ck_r r eqs, *)
+  (*     well_structured_memories (EqCall xs ck f i es :: eqs) M -> *)
+  (*     well_structured_memories (EqReset ck_r f i r :: EqCall xs ck f i es :: eqs) M. *)
+  (* Proof. *)
+  (*   inversion_clear 1 as [Vals Insts]. *)
+  (*   constructor; unfold fbys, insts in *; simpl in *. *)
+  (*   - intro; rewrite Vals; reflexivity. *)
+  (*   - intro; rewrite Insts. *)
+  (*     rewrite 2 In_fold_left_inst_eq. *)
+  (*     split; intros [H|H']; auto. *)
+  (*     + rewrite PSE.MP.Dec.F.add_iff; auto. *)
+  (*     + apply PSE.MP.Dec.F.add_iff in H' as []; auto. *)
+  (*       rewrite PSE.MP.Dec.F.add_iff; auto. *)
+  (* Qed. *)
 
-  Corollary well_structured_add_inst_reset_call:
-    forall M M' xs ck f i es ck_r r eqs,
-      well_structured_memories eqs M ->
-      well_structured_memories (EqReset ck_r f i r :: EqCall xs ck f i es :: eqs) (add_inst i M' M).
-  Proof.
-    intros; apply well_structured_reset_call, well_structured_add_inst_call; auto.
-  Qed.
+  (* Corollary well_structured_add_inst_reset_call: *)
+  (*   forall M M' xs ck f i es ck_r r eqs, *)
+  (*     well_structured_memories eqs M -> *)
+  (*     well_structured_memories (EqReset ck_r f i r :: EqCall xs ck f i es :: eqs) (add_inst i M' M). *)
+  (* Proof. *)
+  (*   intros; apply well_structured_reset_call, well_structured_add_inst_call; auto. *)
+  (* Qed. *)
 
-  Lemma well_structured_add_val_fby:
-    forall M mvs x ck v0 e eqs,
-      well_structured_memories eqs M ->
-      well_structured_memories (EqFby x ck v0 e :: eqs) (add_val x mvs M).
-  Proof.
-    intros ** WS.
-    constructor; unfold fbys, insts; simpl; split; intro H.
-    - rewrite In_fold_left_fby_eq.
-      destruct (ident_eqb x x0) eqn: E;
-        [apply ident_eqb_eq in E; subst|apply ident_eqb_neq in E].
-      + right; apply PSE.MP.Dec.F.add_1; auto.
-      + rewrite find_val_gso in H; auto.
-        apply WS in H; auto.
-    - destruct (ident_eqb x x0) eqn: E;
-        [apply ident_eqb_eq in E; subst|apply ident_eqb_neq in E].
-      + rewrite find_val_gss; intro; discriminate.
-      + rewrite find_val_gso; auto.
-        apply WS.
-        apply In_fold_left_fby_eq in H as [|H]; auto.
-        apply PSE.MP.Dec.F.add_3 in H; auto.
-        contradict H; apply not_In_empty.
-    - rewrite find_inst_add_val in H; apply WS in H; auto.
-    - rewrite find_inst_add_val; apply WS in H; auto.
-  Qed.
+  (* Lemma well_structured_add_val_fby: *)
+  (*   forall M mvs x ck v0 e eqs, *)
+  (*     well_structured_memories eqs M -> *)
+  (*     well_structured_memories (EqFby x ck v0 e :: eqs) (add_val x mvs M). *)
+  (* Proof. *)
+  (*   intros ** WS. *)
+  (*   constructor; unfold fbys, insts; simpl; split; intro H. *)
+  (*   - rewrite In_fold_left_fby_eq. *)
+  (*     destruct (ident_eqb x x0) eqn: E; *)
+  (*       [apply ident_eqb_eq in E; subst|apply ident_eqb_neq in E]. *)
+  (*     + right; apply PSE.MP.Dec.F.add_1; auto. *)
+  (*     + rewrite find_val_gso in H; auto. *)
+  (*       apply WS in H; auto. *)
+  (*   - destruct (ident_eqb x x0) eqn: E; *)
+  (*       [apply ident_eqb_eq in E; subst|apply ident_eqb_neq in E]. *)
+  (*     + rewrite find_val_gss; intro; discriminate. *)
+  (*     + rewrite find_val_gso; auto. *)
+  (*       apply WS. *)
+  (*       apply In_fold_left_fby_eq in H as [|H]; auto. *)
+  (*       apply PSE.MP.Dec.F.add_3 in H; auto. *)
+  (*       contradict H; apply not_In_empty. *)
+  (*   - rewrite find_inst_add_val in H; apply WS in H; auto. *)
+  (*   - rewrite find_inst_add_val; apply WS in H; auto. *)
+  (* Qed. *)
 
 End SBSEMANTICS.
